steel/formats/spec/Zeta.Steel.LogEntry.Spec.fst
@@ -5,3 +5,7 @@ let spec_parser_log_entry = Zeta.Formats.LogEntry.parse_log_entry
 let spec_serializer_log_entry x =
   assert (LowParse.Spec.Base.parse Zeta.Formats.LogEntry.parse_log_entry (Zeta.Formats.LogEntry.serialize_log_entry x) == Some (x, Seq.length (Zeta.Formats.LogEntry.serialize_log_entry x))); // pattern requires `LowParse.Spec.Base.parse`
   Zeta.Formats.LogEntry.serialize_log_entry x
+
+let spec_parser_log_entry_consumes_at_least_one_byte bytes =
+  let _ = LowParse.Spec.Base.parse Zeta.Formats.LogEntry.parse_log_entry bytes in // SMT pattern
+  LowParse.Spec.Base.parser_kind_prop_equiv Zeta.Formats.LogEntry.parse_log_entry_kind Zeta.Formats.LogEntry.parse_log_entry
